Refactor the [int] type to use [val_to_Z]..

theories/typing/atomic_bool.v
@@ -7,34 +7,36 @@ Section atomic_bool.
   Context `{!typeG Σ}.
 
   Program Definition atomic_bool (it : int_type) (PT PF : iProp Σ) : type := {|
-    ty_own β l := (match β return _ with
-                  | Own => ∃ b, l ◁ₗ b @ boolean it ∗ if b then PT else PF
-                  | Shr => ⌜l `has_layout_loc` it⌝ ∗
-                          inv atomic_boolN (∃ b, l ↦ i2v (Z_of_bool b) it ∗ if b then PT else PF)
-                  end)%I
-  |}.
+    ty_own β l :=
+      match β return _ with
+      | Own => ∃ b, l ◁ₗ b @ boolean it ∗ if b then PT else PF
+      | Shr => ⌜l `has_layout_loc` it⌝ ∗
+               inv atomic_boolN (∃ b, l ↦ i2v (Z_of_bool b) it ∗ if b then PT else PF)
+      end;
+  |}%I.
   Next Obligation.
-    iIntros (PT PF l E HE) => /=. iDestruct 1 as (b) "[Hb Hown]".
+    iIntros "%it %PT %PF %l %E %HE (%b&Hb&Hown)".
     iDestruct (ty_aligned with "Hb") as %?. iSplitR => //.
-    iApply inv_alloc. iIntros "!#". iExists b. iFrame.
-    iDestruct (ty_deref with "Hb") as (v) "[Hl Hb]".
-    (* TODO: don't unfold here *)
-    rewrite /i2v. by iDestruct "Hb" as %->.
+    iApply inv_alloc. iNext. iExists b. iFrame.
+    iDestruct (ty_deref with "Hb") as "(%v&Hl&Hb)".
+    by iDestruct (boolean_own_val_eq with "Hb") as %<-.
   Qed.
 
   Global Program Instance movable_atomic_bool it PT PF : Movable (atomic_bool it PT PF) := {|
     ty_layout := it_layout it;
     ty_own_val v := ∃ b, v ◁ᵥ b @ boolean it ∗ if b then PT else PF;
   |}%I.
-  Next Obligation. iIntros (it PT PF l). iDestruct 1 as (?) "[Hb _]". by iApply (ty_aligned with "Hb"). Qed.
-  Next Obligation. iIntros (it PT PF v). iDestruct 1 as (?) "[Hb _]". by iApply (ty_size_eq with "Hb"). Qed.
+  Next Obligation. iIntros (????) "[% [Hb _]]". by iApply (ty_aligned with "Hb"). Qed.
+  Next Obligation. iIntros (????) "[% [Hb _]]". by iApply (ty_size_eq with "Hb"). Qed.
   Next Obligation.
-    iIntros (it PT PF v). iDestruct 1 as (?) "[Hb ?]".
-    iDestruct (ty_deref with "Hb") as (?) "[? ?]". eauto with iFrame.
+    iIntros (????) "[% [Hb ?]]".
+    iDestruct (ty_deref with "Hb") as (?) "[? ?]".
+    eauto with iFrame.
   Qed.
   Next Obligation.
-    iIntros (it PT PF l v ?) "Hl". iDestruct 1 as (?) "[Hb ?]".
-    iDestruct (ty_ref with "[] Hl Hb") as "?" => //. iExists _. iFrame.
+    iIntros (??????) "Hl [%b [Hb ?]]".
+    iDestruct (ty_ref with "[] Hl Hb") as "?" => //.
+    iExists b. iFrame.
   Qed.
 
 End atomic_bool.
@@ -57,29 +59,35 @@ Section programs.
     λ T, i2p (subsume_atomic_bool_own_int l n it PT PF T).
 
   Lemma type_read_atomic_bool l β it PT PF T:
-    (∀ b v, destruct_hint (DHintDestruct bool b) tt ((if b then PT else PF) -∗ (if b then PT else PF) ∗ T v (atomic_bool it PT PF) (t2mt (b @ boolean it)))) -∗
+    (∀ b v,
+      destruct_hint (DHintDestruct bool b) tt (
+        (if b then PT else PF) -∗
+        (if b then PT else PF) ∗
+        T v (atomic_bool it PT PF) (t2mt (b @ boolean it))
+      )
+    ) -∗
     typed_read_end true l β (atomic_bool it PT PF) it T.
   Proof.
-    iIntros "HT Hl". unfold destruct_hint.
-    destruct β.
-    - iDestruct "Hl" as (b) "[Hl Hif]".
+    unfold destruct_hint. iIntros "HT Hl". destruct β.
+    - iDestruct "Hl" as "[%b [Hl Hif]]".
       iApply fupd_mask_intro => //. iIntros "Hclose".
       iDestruct (ty_aligned with "Hl") as %?.
       iDestruct (ty_deref with "Hl") as (v) "[Hl #Hv]".
       iDestruct (ty_size_eq with "Hv") as %?.
-      iExists _, _, _, (t2mt (b @ boolean it)). iFrame "∗Hv". do 2 iSplitR => //=.
+      iExists _, _, _, (t2mt (b @ boolean it)).
+      iFrame "∗Hv". do 2 iSplitR => //=.
       iIntros "!# Hl". iMod "Hclose". iModIntro.
       iDestruct ("HT" with "Hif") as "[Hif $]".
-      iExists b. iFrame.
-        by iApply (ty_ref with "[] Hl Hv").
+      iExists b. iFrame. by iApply (ty_ref with "[] Hl Hv").
     - iDestruct "Hl" as (Hly) "#Hinv".
       iInv "Hinv" as (b) "[>Hl Hif]" "Hclose".
       iApply fupd_mask_intro. set_solver. iIntros "Hclose2".
       iExists _, _, _, (t2mt (b @ boolean it)). iFrame.
       rewrite /has_layout_val i2v_bool_length.
-      do 2 iSplitR => //=. iSplitR => //. { by rewrite /ty_own_val/= val_of_Z_bool. }
+      do 2 iSplitR => //=. iSplitR; first by iApply boolean_own_val_eq.
       iIntros "!# Hl". iDestruct ("HT" with "Hif") as "[Hif $]".
-      iMod "Hclose2" as "_". iMod ("Hclose" with "[-]"). { iExists _. by iFrame. }
+      iMod "Hclose2" as "_".
+      iMod ("Hclose" with "[-]"). { iExists _. by iFrame. }
       iModIntro. by iSplitR.
   Qed.
   Global Instance type_read_atomic_bool_inst l β it PT PF:
@@ -87,13 +95,19 @@ Section programs.
     λ T, i2p (type_read_atomic_bool l β it PT PF T).
 
   Lemma type_write_atomic_bool l β it PT PF v ty `{!Movable ty} T:
-    (∃ b, subsume (v ◁ᵥ ty) (v ◁ᵥ b @ boolean it) (⌜ty.(ty_layout) = it⌝ ∗ (if b then PT else PF) ∗ T (atomic_bool it PT PF))) -∗
+    (∃ b,
+      subsume (v ◁ᵥ ty) (v ◁ᵥ b @ boolean it) (
+        ⌜ty.(ty_layout) = it⌝ ∗
+        (if b then PT else PF) ∗
+        T (atomic_bool it PT PF)
+      )
+    ) -∗
     typed_write_end true v ty l β (atomic_bool it PT PF) T.
   Proof.
-    iIntros "HT Hl Hv". iDestruct "HT" as (bnew) "Hsub".
-    iDestruct ("Hsub" with "Hv") as "(Hnew&->&Hif'&HT)".
+    iIntros "[%bnew Hsub] Hl Hv".
+    iDestruct ("Hsub" with "Hv") as "(Hnew&->&Hif_new&HT)".
     destruct β.
-    - iDestruct "Hl" as (bold) "[Hl Hif]".
+    - iDestruct "Hl" as "[%bold [Hl Hif_old]]".
       iApply fupd_mask_intro => //. iIntros "Hc".
       iDestruct (ty_aligned with "Hl") as %?.
       iDestruct (ty_deref with "Hl") as (vb) "[Hmt Hold]".
@@ -104,12 +118,13 @@ Section programs.
       iApply (@ty_ref with "[] Hl") => //. done.
     - iDestruct "Hl" as (?) "#Hinv".
       iInv "Hinv" as (b) "[>Hmt Hif]" "Hc".
-      iApply fupd_mask_intro; first solve_ndisj. iIntros "Hc2".
-      iSplitL "Hmt".
+      iApply fupd_mask_intro; first solve_ndisj.
+      iIntros "Hc2". iSplitL "Hmt".
       { iExists _; iFrame; iPureIntro; split => //. apply i2v_bool_length. }
       iIntros "!# Hl". iMod "Hc2".
-      iMod ("Hc" with "[Hif' Hl Hnew]").
-      { iModIntro. iExists bnew. iFrame. rewrite /i2v. by iDestruct "Hnew" as %->. }
+      iDestruct (boolean_own_val_eq with "Hnew") as %->.
+      iMod ("Hc" with "[Hif_new Hl]").
+      { iModIntro. iExists bnew. iFrame. }
       iModIntro. iExists _. iFrame. by iSplit.
   Qed.
   Global Instance type_write_atomic_bool_inst l β it PT PF v ty `{!Movable ty}:
@@ -117,37 +132,51 @@ Section programs.
     λ T, i2p (type_write_atomic_bool l β it PT PF v ty T).
 
   Lemma type_cas_atomic_bool (l : loc) β it PT PF lexp Pexp vnew Pnew T:
-    (∃ bexp bnew, subsume Pexp (lexp ◁ₗ bexp @ boolean it) (
-                  subsume Pnew (vnew ◁ᵥ bnew @ boolean it) ( ⌜bytes_per_int it ≤ bytes_per_addr⌝%nat ∗ (
-        ((if bexp then PT else PF) -∗ (if bnew then PT else PF) ∗ (
-            l ◁ₗ{β} atomic_bool it PT PF -∗ lexp ◁ₗ bexp @ boolean it -∗
-              T (val_of_bool true) (t2mt (true @ boolean bool_it)))) ∧
-            (l ◁ₗ{β} atomic_bool it PT PF -∗ lexp ◁ₗ negb bexp @ boolean it -∗
-                             T (val_of_bool false) (t2mt (false @ boolean bool_it)))
-    )))) -∗
+    (∃ bexp bnew,
+      subsume Pexp (lexp ◁ₗ bexp @ boolean it) (
+        subsume Pnew (vnew ◁ᵥ bnew @ boolean it) (
+          ⌜bytes_per_int it ≤ bytes_per_addr⌝%nat ∗ (
+            ((if bexp then PT else PF) -∗
+             (if bnew then PT else PF) ∗ (
+                l ◁ₗ{β} atomic_bool it PT PF -∗ lexp ◁ₗ bexp @ boolean it -∗
+                T (val_of_bool true) (t2mt (true @ boolean bool_it)))) ∧
+            (l ◁ₗ{β} atomic_bool it PT PF -∗
+             lexp ◁ₗ negb bexp @ boolean it -∗
+             T (val_of_bool false) (t2mt (false @ boolean bool_it)))
+           )
+        )
+      )
+    ) -∗
     typed_cas (IntOp it) l (l ◁ₗ{β} (atomic_bool it PT PF))%I lexp Pexp vnew Pnew T.
   Proof.
-    iDestruct 1 as (bexp bnew) "Hsub". iIntros "Hl Hlexp Hvnew".
+    iIntros "(%bexp&%bnew&Hsub) Hl Hlexp Hvnew".
     iDestruct ("Hsub" with "Hlexp") as "[Hlexp Hsub]".
     iDestruct ("Hsub" with "Hvnew") as "[Hvnew [% Hsub]]".
     iIntros (Φ) "HΦ".
     (* TODO: don't unfold here *)
-    rewrite {1 2}/boolean/boolean_inner_type/int_inner_type/=.
+    rewrite {1 2}/boolean/boolean_inner_type/int/int_inner_type/=.
     iDestruct "Hlexp" as (ve Hve Hle) "He" => /=.
     iDestruct "Hvnew" as %Hvnew.
     destruct β.
     - iDestruct "Hl" as (b) "[Hb Hif]".
       (* TODO: don't unfold here *)
-      rewrite {1}/boolean/boolean_inner_type/int_inner_type/=.
+      rewrite {1}/boolean/boolean_inner_type/int/int_inner_type/=.
       iDestruct "Hb" as (vb Hvb Hlb) "Hb" => /=.
       destruct (decide (b = bexp)); subst.
-      + iApply (wp_cas_suc with "Hb He") => //; try by [apply val_to_of_loc]; try by [apply val_to_of_int]; try by [apply: val_of_Z_length].
+      + iApply (wp_cas_suc with "Hb He") => //.
+        { by apply val_to_of_loc. }
+        { by apply val_to_of_loc. }
+        { by eapply val_to_Z_length. }
         iIntros "!# Hb Hexp".
         iDestruct "Hsub" as "[Hsub _]". iDestruct ("Hsub" with "Hif") as "[Hif HT]".
         iApply "HΦ". 2: iApply ("HT" with "[Hb Hif]"). done.
         * iExists bnew. iFrame "Hif". iExists _. by iFrame.
         * iExists _. by iFrame.
-      + iApply (wp_cas_fail with "Hb He") => //; try by [apply val_to_of_loc]; try by [apply val_to_of_int]; try by [apply: val_of_Z_length]; try by [destruct b,bexp].
+      + iApply (wp_cas_fail with "Hb He") => //.
+        { by apply val_to_of_loc. }
+        { by apply val_to_of_loc. }
+        { by eapply val_to_Z_length. }
+        { by destruct b, bexp. }
         iIntros "!# Hb Hexp".
         iDestruct "Hsub" as "[_ HT]".
         iApply "HΦ". 2: iApply ("HT" with "[Hb Hif]"). done.
@@ -157,20 +186,42 @@ Section programs.
       iInv "Hinv" as "Hb".
       iDestruct "Hb" as (b) "[>Hmt Hif]".
       destruct (decide (b = bexp)); subst.
-      + iApply (wp_cas_suc with "Hmt He") => //; try by [apply val_to_of_loc]; try by [apply val_to_of_int]; try by [apply: val_of_Z_length]; try by [apply i2v_bool_Some].
+      + iApply (wp_cas_suc with "Hmt He") => //.
+        { by apply val_to_of_loc. }
+        { by apply val_to_of_loc. }
+        { apply val_to_of_int. rewrite /i2v.
+          have Hin: Z_of_bool bexp ∈ it by apply Z_of_bool_elem_of_int_type.
+          apply val_of_Z_is_some in Hin. destruct Hin as [? ->]. done. }
+        { by eapply val_to_Z_length. }
         iIntros "!# Hb Hexp".
         iDestruct "Hsub" as "[Hsub _]". iDestruct ("Hsub" with "Hif") as "[Hif HT]".
-        iModIntro. iSplitL "Hb Hif". { by iExists bnew; iFrame; rewrite /i2v Hvnew. }
+        iModIntro. iSplitL "Hb Hif".
+        { iExists bnew. iFrame.
+          assert (vnew = i2v (Z_of_bool bnew) it) as ->; last done.
+          rewrite /i2v.
+          have Hin: Z_of_bool bnew ∈ it by apply Z_of_bool_elem_of_int_type.
+          apply val_of_Z_is_some in Hin. destruct Hin as [? Heq]. rewrite Heq /=.
+          apply val_to_of_int in Heq. by eapply val_to_Z_Some_inj. }
         iApply "HΦ". 2: iApply ("HT" with "[]"). done.
         * by iSplit.
         * iExists _. by iFrame.
-      + iApply (wp_cas_fail with "Hmt He") => //; try by [apply val_to_of_loc]; try by [apply val_to_of_int]; try by [apply i2v_bool_Some]; try by [apply: val_of_Z_length]; try by [destruct b,bexp].
+      + iApply (wp_cas_fail with "Hmt He") => //.
+        { by apply val_to_of_loc. }
+        { by apply val_to_of_loc. }
+        { apply val_to_of_int. rewrite /i2v.
+          have Hin: Z_of_bool b ∈ it by apply Z_of_bool_elem_of_int_type.
+          apply val_of_Z_is_some in Hin. destruct Hin as [? ->]. done. }
+        { by eapply val_to_Z_length. }
+        { by destruct b, bexp. }
         iIntros "!# Hb Hexp".
         iDestruct "Hsub" as "[_ HT]".
         iModIntro. iSplitL "Hb Hif". { by iExists b; iFrame; rewrite /i2v Hvnew. }
         iApply "HΦ". 2: iApply ("HT" with "[]"). done.
         * by iSplit.
-        * iExists _. iFrame. rewrite val_of_Z_bool. by destruct b, bexp.
+        * iExists _. iFrame. iSplit; last done. iPureIntro. rewrite /i2v.
+          have Hin: Z_of_bool b ∈ it by apply Z_of_bool_elem_of_int_type.
+          apply val_of_Z_is_some in Hin. destruct Hin as [? Heq]. rewrite Heq /=.
+          apply val_to_of_int in Heq. rewrite Heq. by destruct b, bexp.
   Qed.
   Global Instance type_cas_atomic_bool_inst (l : loc) β it PT PF (lexp : loc) Pexp vnew Pnew:
     TypedCas (IntOp it) l (l ◁ₗ{β} (atomic_bool it PT PF))%I lexp Pexp vnew Pnew :=
