examples/proofs/wrapping_add/wrapping_rules.v
@@ -21,16 +21,16 @@ Section type.
     iDestruct ("HT" with "Hty2") as (Hv2) "HT".
     iIntros (Φ) "HΦ".
     iDestruct ("HT" with "[] []" ) as (??) "HT".
-    1-2: iPureIntro; by apply: val_of_Z_in_range.
+    1-2: iPureIntro; by apply: val_to_Z_in_range.
     have /val_of_Z_is_some[v Hv] : ((n1 + n2) `mod` int_modulus it1) ∈ it1 by apply int_modulus_mod_in_range.
-    move: Hv1 Hv2 => /val_to_of_int Hv1 /val_to_of_int Hv2. subst it2.
+    subst it2.
     iApply (wp_binop_det v). iSplit.
     - iIntros (σ v') "_ !%". split.
       + inversion 1; simplify_eq/=.
         by destruct it1 as [? []]; simplify_eq/=.
       + move => ->. econstructor => //.
         by destruct it1 as [? []]; simplify_eq/=.
-    - iIntros "!>". iApply "HΦ"; last done. by iPureIntro.
+    - iIntros "!>". iApply "HΦ"; last done. iPureIntro. by apply val_to_of_int.
   Qed.
 
   Global Instance macro_wrapping_add_inst it1 it2 e1 e2 :
